\documentclass[10pt]{article}
\usepackage{latexsym}
\usepackage{amsmath}
\usepackage{natbib}
\usepackage{graphicx}
\usepackage{listings}
\usepackage{amssymb} 

\renewcommand{\P}{\mathbb{P}}

\title{MCMT Homework 6}
\author{Shun Zhang}
\date{}

\begin{document}
\maketitle

\section*{Exercise 6.1}

$2 ||\mu P^t - \pi||_{TV} 
= \sum_{y \in \Omega} |(\mu P^t)(y) - \pi (y)| \\
= \sum_{y \in \Omega} |\sum_{x \in \Omega}\mu(x) P^t(x, y) - \pi(y)| \\
= \sum_{y \in \Omega} |\sum_{x \in \Omega}\mu(x) P^t(x, y) - \sum_{x \in
\Omega}\mu(x) \pi(y)| \\
= \sum_{y \in \Omega} |\sum_{x \in \Omega}\mu(x) (P^t(x, y) - \pi(y))| \\
\leq \sum_{y \in \Omega} \sum_{x \in \Omega}\mu(x) |P^t(x, y) - \pi(y)| \\
= \sum_{x \in \Omega}\mu(x) 2||P^t(x, \cdot) - \pi||_{TV} \\
\leq \sup_{x \in \Omega} 2||P^t(x, \cdot) - \pi||_{TV} \\
$

In the last step, we know $\mu(x)$ sums to 1 for $x \in \Omega$. So to maximize
it, let $\mu = \delta_x$ so that $2||P^t(x, \cdot) - \pi||_{TV}$ is maximized.
Therefore, $\sup_\mu ||\mu P^t - \pi||_{TV} = d(t)$.
\\

$2 ||\mu P^t - \nu P^t||_{TV} 
= \sum_{y \in \Omega} |(\mu P^t)(y) - (\nu P^t)(y)| \\
= \sum_{y \in \Omega} |\sum_{x \in \Omega}\mu(x) P^t(x, y) - \sum_{z \in
\Omega}\nu (z) P^t(z, y)| \\
= \sum_{y \in \Omega} |\sum_{x \in \Omega}\mu(x) \sum_{z \in \Omega}\nu (z) (
P^t(x, y) - P^t(z, y))| \\
\leq \sum_{y \in \Omega} \sum_{x \in \Omega}\mu(x) \sum_{z \in \Omega}\nu (z) |
P^t(x, y) - P^t(z, y)| \\
= \sum_{x \in \Omega}\mu(x) \sum_{z \in \Omega}\nu (z) 2|| P^t(x, \cdot) -
P^t(z, \cdot)||_{TV} \\
\leq \sup_{x, z \in \Omega} 2|| P^t(x, \cdot) - P^t(z, \cdot)||_{TV} \\
$

The last step is similar to the reasoning to the previous proof. We choose
$\mu = \delta_x, \nu = \delta_z$ so that $2|| P^t(x, \cdot) - P^t(z,
\cdot)||_{TV}$ is maximized.
Therefore,  $\sup_{\mu, \nu} ||\mu P^t - \nu P^t||_{TV} = \bar{d}(t)$.

\section*{Exercise 6.2}

$2 ||\mu P - \nu P||_{TV} 
= \sum_{y \in \Omega} |(\mu P)(y) - (\nu P)(y)| \\
= \sum_{y \in \Omega} |\sum_{x \in \Omega} (\mu(x) P(x, y) - \nu(x) P(x, y))| \\
\leq \sum_{y \in \Omega} \sum_{x \in \Omega} |\mu(x) P(x, y) - \nu(x) P(x, y)| \\
= \sum_{y \in \Omega} \sum_{x \in \Omega} P(x, y) |\mu(x) - \nu(x)| \\
= \sum_{x \in \Omega} |\mu(x) - \nu(x)| \hfill \sum_{y \in \Omega} P(x, y) = 1  \\
= 2 ||\mu - \nu||_{TV} \\
$

So $||\mu P - \nu P||_{TV} \leq ||\mu - \nu||_{TV}$. We have $||\mu P^{t+1} -
\nu P^{t+1}||_{TV} \leq ||\mu P^t - \nu P^t||_{TV}$ by substituting $\mu, \nu$
in the proof above by $\mu P^t, \nu P^t$, respectively.  So we have $\bar{d}(t +
1) \leq \bar{d}(t)$.

We have $||\mu P^{t+1} - \pi||_{TV} \leq ||\mu P^t - \pi||_{TV}$ by
substituting $\mu, \nu$ in the proof above by $\mu P^t, \pi$, respectively. Note
that $\pi P = \pi$.  So we have $\bar{d}(t + 1) \leq \bar{d}(t)$.

\end{document}
