\documentclass[10pt]{article}
\usepackage{latexsym}
\usepackage{amsmath}
\usepackage{natbib}
\usepackage{graphicx}
\usepackage{listings}
\usepackage{amssymb} 
\usepackage{enumerate}

\renewcommand{\P}{\mathbb{P}}
\newcommand{\Cov}{\mathrm{Cov}}
\newcommand{\E}{\mathrm{E}}
\newcommand{\Var}{\mathrm{Var}}

\title{MCMT Homework 12}
\author{Shun Zhang}
\date{}

\begin{document}
\maketitle

\section*{Exercise 12.1}
$\theta(x, y) = -\theta(y, x)$ for every x, y, so $\sum_x \sum_{y \sim x}
\theta(x, y) = 0$. We know for every $x \not\in \{a,z\}$, $\sum_{y \sim x}
\theta(x,y)=0$. So $\sum_{x \in \{a, z\}} \sum_{y \sim x} \theta(x, y) = 0$. 
$\sum_{y \sim a} \theta(a,y)= -\sum_{y \sim z} \theta(z,y)$.

\section*{Exercise 12.2}
Let $\theta$ be the unit current flow of the original graph.

\begin{enumerate}[(a)]
\item
$\sum_{y \sim u} \theta(u, y) =
\sum_{y \sim u} c(u, y) (\phi(u) - \phi(y)) =
(c(e_1) + c(e_2)) (\phi(u) - \phi(v)) + \sum_{y \sim u \setminus \{e_1, e_2\}}
c(u, y) (\phi(u) - \phi(y)) = 0
$.

Delete $e_2$ and replace $c(e_1)$ with $c(e_1)+c(e_2)$. The equation above is
not changed. As $c$ is unchanged for other edges, $\phi$ is the same. By the
definition of $R(a, z) = \phi(a) - \phi(z)$, $R(a, z)$ is the same.

\item
By Kirchoffâ€™s node law, $\theta(v, u) = - \theta(v, w)$. So $\theta(u, v) =
\theta(v, w)$.

$\phi(u) - \phi(w) = (\phi(u) - \phi(v)) + (\phi(v) - \phi(w)) = \theta(u, v)
R(u, v) + \theta(v, w) R(v, w) = \theta(u, v) (R(u, v) + R(v, w))$.

Replace $R(u, v) + R(v, w)$ with $R(u, w)$, $\phi(u) - \phi(w)$ is the same.
Same as the reasoning in previous question, $R(a, z)$ is the same.
\end{enumerate}
\end{document}
